angelic-designs/utp_ades_ops.thy
@@ -108,6 +108,98 @@ lemma aseq_assoc:
   "((P ;;\<^sub>A Q) ;;\<^sub>A R) = (P ;;\<^sub>A (Q ;;\<^sub>A R))"
   by (simp add: aseq_def fun_eq_iff)
 
+subsection \<open>Full-alphabet Angelic Sequential Composition\<close>
+
+text \<open>
+  The operator below lifts angelic relation composition to the complete
+  design alphabet.  It threads the state and angelic-choice components while
+  leaving the two \<open>ok\<close> observations unchanged.
+\<close>
+
+definition aseq_ades ::
+  "'s angelic_design \<Rightarrow> 's angelic_design \<Rightarrow> 's angelic_design"
+  (infixl ";;\<^sub>A\<^sub>D" 75)
+where [pred]: "P ;;\<^sub>A\<^sub>D Q = (\<lambda> (s0, ac').
+  P (s0, des_vars.more_update
+    (achoices.ac\<^sub>v_update (\<lambda>_.
+      {s1. Q (des_vars.more_update
+        (astate.s\<^sub>v_update (\<lambda>_. s1)) s0, ac')})) ac'))"
+
+(* Embedding angelic relations as designs preserves sequential composition. *)
+lemma arel_to_ades_aseq:
+  "arel_to_ades (P ;;\<^sub>A Q) =
+   (arel_to_ades P ;;\<^sub>A\<^sub>D arel_to_ades Q)"
+  by (simp add: arel_to_ades_def rdesign_def design_def
+      aseq_def aseq_ades_def fun_eq_iff; pred_auto)
+
+lemma aseq_ades_true_left [simp]: "true ;;\<^sub>A\<^sub>D P = true"
+  by pred_auto
+
+lemma aseq_ades_false_left [simp]: "false ;;\<^sub>A\<^sub>D P = false"
+  by pred_auto
+
+lemma aseq_ades_disj_distrib:
+  "((P \<or> Q) ;;\<^sub>A\<^sub>D R) = ((P ;;\<^sub>A\<^sub>D R) \<or> (Q ;;\<^sub>A\<^sub>D R))"
+  by pred_auto
+
+lemma aseq_ades_mono_left:
+  "P \<sqsubseteq> Q \<Longrightarrow> (P ;;\<^sub>A\<^sub>D R) \<sqsubseteq> (Q ;;\<^sub>A\<^sub>D R)"
+  by (auto simp add: aseq_ades_def pred_refine_iff split: prod.splits)
+
+(* The paper's s \<in> ac' lifted to the full design alphabet. *)
+definition ades_state_choice :: "'s angelic_design" where
+[pred]: "ades_state_choice = (\<lambda> (s0, ac').
+  astate.s\<^sub>v (des_vars.more s0) \<in> achoices.ac\<^sub>v (des_vars.more ac'))"
+
+lemma aseq_ades_state_choice_left [simp]:
+  "(ades_state_choice ;;\<^sub>A\<^sub>D P) = P"
+  by pred_auto
+
+(* The two fields of the design observation can be updated independently. *)
+lemma des_more_ok_update_commute:
+  "des_vars.more_update f (ok\<^sub>v_update g r) =
+   ok\<^sub>v_update g (des_vars.more_update f r)"
+  by (cases r) simp
+
+lemma aseq_ades_unrest_ok_out [unrest]:
+  "\<lbrakk> $ok\<^sup>> \<sharp> P; $ok\<^sup>> \<sharp> Q \<rbrakk> \<Longrightarrow>
+   $ok\<^sup>> \<sharp> (P ;;\<^sub>A\<^sub>D Q)"
+  apply (simp add: unrest_lens aseq_ades_def)
+  apply (simp add: subst_app_def subst_upd_def subst_id_def
+      SEXP_def lens_defs alpha_defs des_more_ok_update_commute)
+  done
+
+lemma aseq_ades_unrest_ok_in [unrest]:
+  "\<lbrakk> $ok\<^sup>< \<sharp> P; $ok\<^sup>< \<sharp> Q \<rbrakk> \<Longrightarrow>
+   $ok\<^sup>< \<sharp> (P ;;\<^sub>A\<^sub>D Q)"
+  apply (simp add: unrest_lens aseq_ades_def)
+  apply (simp add: subst_app_def subst_upd_def subst_id_def
+      SEXP_def lens_defs alpha_defs)
+  apply (simp add: des_more_ok_update_commute)
+  done
+
+lemma ades_state_choice_unrest_ok_out [unrest]:
+  "$ok\<^sup>> \<sharp> (ades_state_choice :: 's angelic_design)"
+  apply (simp add: unrest_lens ades_state_choice_def)
+  apply (simp add: subst_app_def subst_upd_def subst_id_def
+      SEXP_def lens_defs alpha_defs)
+  done
+
+lemma ades_state_choice_unrest_ok_in [unrest]:
+  "$ok\<^sup>< \<sharp> (ades_state_choice :: 's angelic_design)"
+  apply (simp add: unrest_lens ades_state_choice_def)
+  apply (simp add: subst_app_def subst_upd_def subst_id_def
+      SEXP_def lens_defs alpha_defs)
+  done
+
+lemma pred_true_unrest_ok_out [unrest]:
+  "$ok\<^sup>> \<sharp> (true :: 's angelic_design)"
+  by (simp add: unrest_lens; pred_auto)
+
+lemma pred_true_unrest_ok_in [unrest]:
+  "$ok\<^sup>< \<sharp> (true :: 's angelic_design)"
+  by (simp add: unrest_lens; pred_auto)
+
 subsection \<open>Angelic Design Sequential Composition\<close>
 
 (* Paper Definition 18: compose angelic designs through a hidden intermediate ok value. *)
@@ -115,10 +207,92 @@ definition angelic_design_seq ::
   "'s angelic_design \<Rightarrow> 's angelic_design \<Rightarrow> 's angelic_design" (infixl ";;\<^sub>D\<^sub>A" 75)
 where
 [pred]: "angelic_design_seq P Q = (\<lambda> (s0, ac'). \<exists> ok0.
-  P (s0, put\<^bsub>ok\<^esub> (put\<^bsub>\<^bold>v\<^sub>D\<^esub> ac'
-    (put\<^bsub>ac\<^esub> (des_vars.more ac')
-      {s1. Q (put\<^bsub>ok\<^esub> (put\<^bsub>\<^bold>v\<^sub>D\<^esub> s0
-        (put\<^bsub>s\<^esub> (des_vars.more s0) s1)) ok0, ac')})) ok0))"
+  P (s0, ok\<^sub>v_update (\<lambda>_. ok0)
+    (des_vars.more_update (achoices.ac\<^sub>v_update (\<lambda>_.
+        {s1. Q (ok\<^sub>v_update (\<lambda>_. ok0)
+          (des_vars.more_update (astate.s\<^sub>v_update (\<lambda>_. s1)) s0), ac')})) ac')))"
+
+(* Splitting the hidden intermediate observation into its two Boolean cases
+   connects the design operator above to full-alphabet angelic composition. *)
+lemma angelic_design_seq_ok_cases:
+  "P ;;\<^sub>D\<^sub>A Q =
+   ((P\<lbrakk>True/ok\<^sup>>\<rbrakk> ;;\<^sub>A\<^sub>D Q\<lbrakk>True/ok\<^sup><\<rbrakk>) \<or>
+    (P\<lbrakk>False/ok\<^sup>>\<rbrakk> ;;\<^sub>A\<^sub>D Q\<lbrakk>False/ok\<^sup><\<rbrakk>))"
+  by (simp add: angelic_design_seq_def aseq_ades_def fun_eq_iff
+      ex_bool_eq subst_app_def subst_upd_def subst_id_def SEXP_def
+      lens_defs des_vars.ok_def; pred_auto)
+
+subsubsection \<open>Design-observation substitution laws\<close>
+
+lemma design_ok_out_true_subst:
+  assumes "$ok\<^sup>> \<sharp> P" "$ok\<^sup>> \<sharp> Q"
+  shows "(P \<turnstile> Q)\<lbrakk>True/ok\<^sup>>\<rbrakk> = ((\<not> ok\<^sup><) \<or> (\<not> P) \<or> Q)"
+  using assms
+  by (simp add: design_def usubst usubst_eval; pred_auto)
+
+lemma design_ok_out_false_subst:
+  assumes "$ok\<^sup>> \<sharp> P"
+  shows "(P \<turnstile> Q)\<lbrakk>False/ok\<^sup>>\<rbrakk> = ((\<not> ok\<^sup><) \<or> (\<not> P))"
+  using assms
+  by (simp add: design_def usubst usubst_eval; pred_auto)
+
+lemma design_ok_in_true_subst:
+  assumes "$ok\<^sup>< \<sharp> R" "$ok\<^sup>< \<sharp> S"
+  shows "(R \<turnstile> S)\<lbrakk>True/ok\<^sup><\<rbrakk> = ((\<not> R) \<or> (S \<and> ok\<^sup>>))"
+  using assms
+  by (simp add: design_def usubst usubst_eval; pred_auto)
+
+lemma design_ok_in_false_subst:
+  "(R \<turnstile> S)\<lbrakk>False/ok\<^sup><\<rbrakk> = true"
+  by (simp add: design_def fun_eq_iff subst_app_def
+      subst_upd_def subst_id_def SEXP_def lens_defs des_vars.ok_def;
+      pred_auto)
+
+lemma aseq_ades_ok_in_subst:
+  "(P ;;\<^sub>A\<^sub>D Q)\<lbrakk>\<guillemotleft>b\<guillemotright>/ok\<^sup><\<rbrakk> =
+   (P\<lbrakk>\<guillemotleft>b\<guillemotright>/ok\<^sup><\<rbrakk> ;;\<^sub>A\<^sub>D Q\<lbrakk>\<guillemotleft>b\<guillemotright>/ok\<^sup><\<rbrakk>)"
+  by (simp add: aseq_ades_def fun_eq_iff subst_app_def subst_upd_def
+      subst_id_def SEXP_def lens_defs des_vars.ok_def
+      des_more_ok_update_commute; pred_auto)
+
+lemma ok_false_subst_unrest_ok_out [unrest]:
+  "$ok\<^sup>> \<sharp> ((P :: 's angelic_design)\<^sup>f)"
+  apply (simp add: unrest_lens)
+  apply (simp add: subst_app_def subst_upd_def subst_id_def
+      SEXP_def lens_defs alpha_defs des_more_ok_update_commute)
+  done
+
+lemma ok_true_subst_unrest_ok_out [unrest]:
+  "$ok\<^sup>> \<sharp> ((P :: 's angelic_design)\<^sup>t)"
+  apply (simp add: unrest_lens)
+  apply (simp add: subst_app_def subst_upd_def subst_id_def
+      SEXP_def lens_defs alpha_defs des_more_ok_update_commute)
+  done
+
+lemma ok_in_subst_unrest_ok_in [unrest]:
+  "$ok\<^sup>< \<sharp>
+   ((P :: 's angelic_design)\<lbrakk>\<guillemotleft>b\<guillemotright>/ok\<^sup><\<rbrakk>)"
+  apply (simp add: unrest_lens)
+  apply (simp add: subst_app_def subst_upd_def subst_id_def
+      SEXP_def lens_defs alpha_defs)
+  done
+
+lemma state_choice_ok_in_subst [usubst]:
+  "ades_state_choice\<lbrakk>\<guillemotleft>b\<guillemotright>/ok\<^sup><\<rbrakk> = ades_state_choice"
+  by (simp add: ades_state_choice_def fun_eq_iff subst_app_def
+      subst_upd_def subst_id_def SEXP_def lens_defs; pred_auto)
+
+lemma pred_true_ok_in_subst [usubst]:
+  "(true :: 's angelic_design)\<lbrakk>\<guillemotleft>b\<guillemotright>/ok\<^sup><\<rbrakk> = true"
+  by (simp add: fun_eq_iff subst_app_def subst_upd_def
+      subst_id_def SEXP_def lens_defs; pred_auto)
+
+lemma subst_ok_in_absorb [simp]:
+  "((P :: 's angelic_design)\<lbrakk>\<guillemotleft>b\<guillemotright>/ok\<^sup><\<rbrakk>)
+      \<lbrakk>\<guillemotleft>c\<guillemotright>/ok\<^sup><\<rbrakk> =
+   P\<lbrakk>\<guillemotleft>b\<guillemotright>/ok\<^sup><\<rbrakk>"
+  by (simp add: fun_eq_iff subst_app_def subst_upd_def
+      subst_id_def SEXP_def lens_defs; pred_auto)
 
 (* Thesis Theorem T.4.5.1: pre/postcondition form. *)
 definition angelic_design_seq_simplified ::
