utp_rad_nd.thy
@@ -1,13 +1,12 @@
 section \<open>Non-Divergent Reactive Angelic Designs\<close>
 
 theory utp_rad_nd
-  imports utp_rad_ops
+  imports utp_rad_seq
 begin
 
 (* Paper Definition 45: the angelic choice with the most nondeterministic
    non-divergent process. *)
-definition NDRAD ::
-  "'e reactive_angelic_design \<Rightarrow> 'e reactive_angelic_design" where
+definition NDRAD :: "'e reactive_angelic_design \<Rightarrow> 'e reactive_angelic_design" where
 [pred]: "NDRAD P = P \<squnion>\<^sub>R\<^sub>A\<^sub>D Choice\<^sub>R\<^sub>A\<^sub>D"
 
 lemma NDRAD_idem: "NDRAD (NDRAD P) = NDRAD P"
@@ -37,6 +36,46 @@ theorem NDRAD_design_form:
   shows "NDRAD P = (RA \<circ> A) (true \<turnstile> (P \<^sub>wf)\<^sup>t)"
   using Choice_RAD_angelic_choice[OF assms]
   by (simp add: NDRAD_def inf_commute)
+
+(* Paper Theorem 35 / thesis T.5.5.3. The quantifier closes over all
+   observations; the (\<not> ok\<^sup><) disjunct makes the not-started case vacuous,
+   mirroring the thesis' case analysis on initial ok. *)
+theorem NDRAD_fixed_point:
+  assumes "P is RAD"
+  shows "NDRAD P = P \<longleftrightarrow>
+    (\<forall>s0 ac'. ((\<not> ok\<^sup><) \<or> (\<not> (P \<^sub>wf)\<^sup>f)) (s0, ac'))"
+proof
+  assume fixed: "NDRAD P = P"
+  have "((NDRAD P) \<^sub>wf)\<^sup>f\<lbrakk>True/ok\<^sup><\<rbrakk> =
+      ((P \<^sub>wf)\<^sup>f\<lbrakk>True/ok\<^sup><\<rbrakk> \<and>
+       (Choice\<^sub>R\<^sub>A\<^sub>D \<^sub>wf)\<^sup>f\<lbrakk>True/ok\<^sup><\<rbrakk>)"
+    unfolding NDRAD_def RAD_angelic_choice
+    by (simp only: rad_wait_false_conj usubst)
+  also have "... = false"
+    by (simp only: Choice_RAD_wf_ok_false_subst; pred_auto)
+  finally have failure_false:
+      "(P \<^sub>wf)\<^sup>f\<lbrakk>True/ok\<^sup><\<rbrakk> = false"
+    by (simp only: fixed)
+  show "\<forall>s0 ac'.
+      ((\<not> ok\<^sup><) \<or> (\<not> (P \<^sub>wf)\<^sup>f)) (s0, ac')"
+    using failure_false
+    by (simp add: fun_eq_iff usubst usubst_eval; pred_auto)
+next
+  assume nondiv:
+    "\<forall>s0 ac'.
+      ((\<not> ok\<^sup><) \<or> (\<not> (P \<^sub>wf)\<^sup>f)) (s0, ac')"
+  have guard_true:
+      "(\<not> (P \<^sub>wf)\<^sup>f)\<lbrakk>True/ok\<^sup><\<rbrakk> = true"
+    using nondiv
+    by (simp add: fun_eq_iff usubst usubst_eval; pred_auto)
+  have design_eq:
+      "((\<not> (P \<^sub>wf)\<^sup>f) \<turnstile> (P \<^sub>wf)\<^sup>t) =
+       (true \<turnstile> (P \<^sub>wf)\<^sup>t)"
+    by (metis design_subst_ok guard_true pred_true_ok_in_subst)
+  show "NDRAD P = P"
+    by (simp only: NDRAD_design_form[OF assms] design_eq[symmetric]
+        RAD_design_form'[OF assms, symmetric])
+qed
 
 (* Paper Example 20: divergence is avoided at the bottom of the lattice. *)
 lemma NDRAD_Chaos:
