utp_rad_ops.thy
@@ -4,6 +4,46 @@ theory utp_rad_ops
   imports utp_rad_csp
 begin
 
+subsection \<open>Singleton Angelic Choice\<close>
+
+(* An A2-healthy process admits a single agreed final state whenever
+   its postcondition projection holds of an inhabited choice set. *)
+lemma A2_wf_ok_true_singleton_reduce:
+  assumes "P is A2"
+  shows "\<in>\<^sub>a\<^sub>c((P \<^sub>wf)\<^sup>t) \<sqsubseteq>
+    (((P \<^sub>wf)\<^sup>t) \<and> ac_non_empty)"
+proof -
+  have fixed: "A2 P = P"
+    using assms by (simp add: Healthy_def')
+  have "\<in>\<^sub>a\<^sub>c(((A2 P) \<^sub>wf)\<^sup>t) \<sqsubseteq>
+      ((((A2 P) \<^sub>wf)\<^sup>t) \<and> ac_non_empty)"
+    apply (simp add: A2_def ades_singleton_choice_def ac_non_empty_def
+        rad_wait_false_def A2_rel_eq_expanded A2_rel_expanded_def
+        pred_refine_iff fun_eq_iff usubst usubst_eval Let_def)
+    by (pred_auto; blast)
+  then show ?thesis
+    by (simp only: fixed)
+qed
+
+(* PBMH upward closure: the singleton choice is weaker than the
+   full choice set. *)
+lemma ades_singleton_choice_weaken:
+  assumes "T is PBMH_ades"
+  shows "T \<sqsubseteq> \<in>\<^sub>a\<^sub>c(T)"
+  using assms
+  apply (simp add: Healthy_def' PBMH_ades_def PBMH_def pbmh_step_def
+      ades_singleton_choice_def pred_refine_iff fun_eq_iff Let_def)
+  by (pred_auto; blast)
+
+lemma RA1_singleton_absorb:
+  assumes "T is PBMH_ades"
+    and "\<in>\<^sub>a\<^sub>c(T) \<sqsubseteq> (T \<and> ac_non_empty)"
+  shows "RA1 (\<in>\<^sub>a\<^sub>c(T)) = RA1 T"
+  using RA1_mono[OF assms(2)]
+    RA1_mono[OF ades_singleton_choice_weaken[OF assms(1)]]
+  by (simp add: pred_ba.inf_commute RA1_ac_non_empty_absorb
+      pred_refine_iff fun_eq_iff; pred_auto)
+
 subsection \<open>Angelic Choice\<close>
 
 (* Paper Definition 37. *)
@@ -241,6 +281,35 @@ lemma Choice_RAD_is_RAD [closure]: "Choice\<^sub>R\<^sub>A\<^sub>D is RAD"
   unfolding Choice_RAD_def
   by rad_closure
 
+(* Choice_RAD can only fail to stabilise when it has not started. *)
+lemma Choice_RAD_wf_ok_false:
+  "(Choice\<^sub>R\<^sub>A\<^sub>D \<^sub>wf)\<^sup>f = RA2 (RA1 (\<not> ok\<^sup><))"
+proof -
+  have design_norm:
+      "((\<not> (ok\<^sup>> \<^sub>wf)\<^sup>f) \<turnstile> (ok\<^sup>> \<^sub>wf)\<^sup>t) = (true \<turnstile> true)"
+    by (simp add: rad_wait_false_def usubst usubst_eval; pred_auto)
+  have disj_norm:
+      "((\<not> ok\<^sup><) \<or> (ok\<^sup>> \<^sub>wf)\<^sup>f) = (\<not> ok\<^sup><)"
+    by (simp add: rad_wait_false_def usubst usubst_eval; pred_auto)
+  have "((rad_wait_false \<circ> RA \<circ> A) (true \<turnstile> true))\<^sup>f =
+      (RA2 \<circ> RA1 \<circ> PBMH_ades) ((\<not> ok\<^sup><) \<or> (ok\<^sup>> \<^sub>wf)\<^sup>f)"
+    using RA_design_wf_ok_false[of "ok\<^sup>>"]
+    by (simp only: design_norm)
+  then show ?thesis
+    by (simp only: Choice_RAD_alt disj_norm comp_apply PBMH_ades_not_ok_expr)
+qed
+
+lemma Choice_RAD_wf_ok_false_subst:
+  "(Choice\<^sub>R\<^sub>A\<^sub>D \<^sub>wf)\<^sup>f\<lbrakk>True/ok\<^sup><\<rbrakk> = false"
+proof -
+  have not_true: "(\<not> (True)\<^sub>e :: 'e reactive_angelic_design) = false"
+    by pred_auto
+  show ?thesis
+    apply (simp only: Choice_RAD_wf_ok_false RA2_ok_in_subst RA1_ok_in_subst)
+    apply (simp add: usubst usubst_eval)
+    by (simp only: not_true RA1_false RA2_false)
+qed
+
 (* Paper Theorem 26. *)
 theorem Choice_RAD_angelic_choice:
   assumes "P is RAD"
@@ -304,10 +373,10 @@ subsection \<open>Stop\<close>
 
 (* \<exists> y \<in> ac' \<bullet> y.tr = s.tr \<and> y.wait *)
 definition stop_post :: "'e reactive_angelic_design" where
-[pred]: "stop_post = (\<lambda> (x, y).
-  \<exists> z \<in> achoices.ac\<^sub>v (des_vars.more y).
-    rad_state.tr\<^sub>v z = rad_state.tr\<^sub>v (astate.s\<^sub>v (des_vars.more x)) \<and>
-    rad_state.wait\<^sub>v z)"
+[pred]: "stop_post = (\<lambda> (s0, ac').
+  \<exists> y \<in> achoices.ac\<^sub>v (des_vars.more ac').
+    rad_state.tr\<^sub>v y = rad_state.tr\<^sub>v (astate.s\<^sub>v (des_vars.more s0)) \<and>
+    rad_state.wait\<^sub>v y)"
 
 (* Paper Definition 41. *)
 definition Stop_RAD :: "'e reactive_angelic_design" ("Stop\<^sub>R\<^sub>A\<^sub>D") where
@@ -335,6 +404,119 @@ lemma stop_post_unrest_ok [unrest]: "$ok\<^sup>> \<sharp> stop_post"
       SEXP_def lens_defs alpha_defs)
   done
 
+lemma stop_post_unrest_ok_in [unrest]: "$ok\<^sup>< \<sharp> stop_post"
+  apply (simp add: unrest_lens stop_post_def)
+  apply (simp add: subst_app_def subst_upd_def subst_id_def
+      SEXP_def lens_defs alpha_defs)
+  done
+
+(* The Stop postcondition only relates the traces of the initial and
+   final states, so trace normalisation leaves it fixed. *)
+lemma RA2_stop_post: "RA2 stop_post = stop_post"
+  by (simp add: RA2_def stop_post_def rad_normalise_choices_def
+      rad_trace_difference_def rad_zero_trace_def fun_eq_iff Let_def;
+      pred_auto; force)
+
+lemma stop_post_ok_in_subst [usubst]:
+  "stop_post\<lbrakk>\<guillemotleft>b\<guillemotright>/ok\<^sup><\<rbrakk> = stop_post"
+  by (simp add: stop_post_def fun_eq_iff subst_app_def subst_upd_def
+      subst_id_def SEXP_def lens_defs des_vars.ok_def
+      astate.s_def des_vars.more\<^sub>L_def)
+
+lemma stop_post_ok_out_subst [usubst]:
+  "stop_post\<lbrakk>\<guillemotleft>b\<guillemotright>/ok\<^sup>>\<rbrakk> = stop_post"
+  by (simp add: stop_post_def fun_eq_iff subst_app_def subst_upd_def
+      subst_id_def SEXP_def lens_defs des_vars.ok_def
+      astate.s_def des_vars.more\<^sub>L_def)
+
+(* Component normal forms of the design body \<open>stop_post \<and> ok\<^sup>>\<close>
+   witnessing Stop's projections. *)
+lemma stop_design_wf_norm:
+  "((stop_post \<and> ok\<^sup>>) \<^sub>wf) = (stop_post \<and> ok\<^sup>>)"
+  by (simp only: rad_wait_false_conj rad_wait_false_stop_post
+      rad_wait_false_ok_out)
+
+lemma stop_design_ok_false: "(stop_post \<and> ok\<^sup>>)\<^sup>f = false"
+  by (simp add: usubst usubst_eval; pred_auto)
+
+lemma stop_design_ok_true: "(stop_post \<and> ok\<^sup>>)\<^sup>t = stop_post"
+  by (simp add: usubst usubst_eval; pred_auto)
+
+(* Stop can only fail to stabilise when it has not started. *)
+lemma Stop_RAD_wf_ok_false:
+  "(Stop\<^sub>R\<^sub>A\<^sub>D \<^sub>wf)\<^sup>f = RA2 (RA1 (\<not> ok\<^sup><))"
+proof -
+  have design_norm:
+      "((\<not> ((stop_post \<and> ok\<^sup>>) \<^sub>wf)\<^sup>f) \<turnstile>
+        ((stop_post \<and> ok\<^sup>>) \<^sub>wf)\<^sup>t) =
+       (true \<turnstile> stop_post)"
+    by (simp only: stop_design_wf_norm stop_design_ok_false
+        stop_design_ok_true pred_ba.compl_bot_eq)
+  have disj_norm:
+      "((\<not> ok\<^sup><) \<or> ((stop_post \<and> ok\<^sup>>) \<^sub>wf)\<^sup>f) = (\<not> ok\<^sup><)"
+    by (simp only: stop_design_wf_norm stop_design_ok_false
+        pred_ba.sup_bot_right)
+  have "((rad_wait_false \<circ> RA \<circ> A) (true \<turnstile> stop_post))\<^sup>f =
+      (RA2 \<circ> RA1 \<circ> PBMH_ades)
+        ((\<not> ok\<^sup><) \<or> ((stop_post \<and> ok\<^sup>>) \<^sub>wf)\<^sup>f)"
+    using RA_design_wf_ok_false[of "stop_post \<and> ok\<^sup>>"]
+    by (simp only: design_norm)
+  then show ?thesis
+    by (simp only: Stop_RAD_def comp_apply disj_norm
+        PBMH_ades_not_ok_expr)
+qed
+
+lemma Stop_RAD_wf_ok_false_subst:
+  "(Stop\<^sub>R\<^sub>A\<^sub>D \<^sub>wf)\<^sup>f\<lbrakk>True/ok\<^sup><\<rbrakk> = false"
+proof -
+  have not_true: "(\<not> (True)\<^sub>e :: 'e reactive_angelic_design) = false"
+    by pred_auto
+  show ?thesis
+    apply (simp only: Stop_RAD_wf_ok_false RA2_ok_in_subst
+        RA1_ok_in_subst)
+    apply (simp add: usubst usubst_eval)
+    by (simp only: not_true RA1_false RA2_false)
+qed
+
+lemma Stop_RAD_wf_ok_true:
+  "(Stop\<^sub>R\<^sub>A\<^sub>D \<^sub>wf)\<^sup>t = RA2 (RA1 ((\<not> ok\<^sup><) \<or> stop_post))"
+proof -
+  have design_norm:
+      "((\<not> ((stop_post \<and> ok\<^sup>>) \<^sub>wf)\<^sup>f) \<turnstile>
+        ((stop_post \<and> ok\<^sup>>) \<^sub>wf)\<^sup>t) =
+       (true \<turnstile> stop_post)"
+    by (simp only: stop_design_wf_norm stop_design_ok_false
+        stop_design_ok_true pred_ba.compl_bot_eq)
+  have disj_norm:
+      "((\<not> ok\<^sup><) \<or> ((stop_post \<and> ok\<^sup>>) \<^sub>wf)\<^sup>f \<or>
+        ((stop_post \<and> ok\<^sup>>) \<^sub>wf)\<^sup>t) =
+       ((\<not> ok\<^sup><) \<or> stop_post)"
+    by (simp only: stop_design_wf_norm stop_design_ok_false
+        stop_design_ok_true pred_ba.sup_bot_left)
+  have PBMH_norm:
+      "PBMH_ades ((\<not> ok\<^sup><) \<or> stop_post) = ((\<not> ok\<^sup><) \<or> stop_post)"
+    by (simp add: PBMH_ades_disj)
+  have "((rad_wait_false \<circ> RA \<circ> A) (true \<turnstile> stop_post))\<^sup>t =
+      (RA2 \<circ> RA1 \<circ> PBMH_ades)
+        ((\<not> ok\<^sup><) \<or> ((stop_post \<and> ok\<^sup>>) \<^sub>wf)\<^sup>f \<or>
+         ((stop_post \<and> ok\<^sup>>) \<^sub>wf)\<^sup>t)"
+    using RA_design_wf_ok_true[of "stop_post \<and> ok\<^sup>>"]
+    by (simp only: design_norm)
+  then show ?thesis
+    by (simp only: Stop_RAD_def comp_apply disj_norm PBMH_norm)
+qed
+
+lemma Stop_RAD_wf_ok_true_subst:
+  "(Stop\<^sub>R\<^sub>A\<^sub>D \<^sub>wf)\<^sup>t\<lbrakk>True/ok\<^sup><\<rbrakk> = RA2 (RA1 stop_post)"
+proof -
+  have subst_norm:
+      "((\<not> ok\<^sup><) \<or> stop_post)\<lbrakk>True/ok\<^sup><\<rbrakk> = stop_post"
+    by (simp add: usubst usubst_eval; pred_auto)
+  show ?thesis
+    by (simp only: Stop_RAD_wf_ok_true RA2_ok_in_subst
+        RA1_ok_in_subst subst_norm)
+qed
+
 lemma stop_design_is_H [closure]: "(true \<turnstile> stop_post) is \<^bold>H"
   by (rule design_is_H1_H2; simp add: unrest)
 
@@ -344,12 +526,16 @@ lemma Stop_RAD_is_RAD [closure]: "Stop\<^sub>R\<^sub>A\<^sub>D is RAD"
    apply (rule stop_design_is_H)
   by (simp add: rad_wait_false_distrib rad_wait_false_stop_post)
 
+(* Stop with the A absorbed into RA. *)
+lemma Stop_RAD_RA: "Stop\<^sub>R\<^sub>A\<^sub>D = RA (true \<turnstile> stop_post)"
+  unfolding Stop_RAD_def
+  by (rule RA_A_absorb_design_true; simp add: Healthy_def' unrest)
+
 (* Paper Theorem 28. *)
 theorem Stop_RAD_angelic_choice:
   assumes "P is RAD"
   shows "Stop\<^sub>R\<^sub>A\<^sub>D \<squnion>\<^sub>R\<^sub>A\<^sub>D P =
-    (RA \<circ> A) (true \<turnstile>
-      (((\<not> (P \<^sub>wf)\<^sup>f) \<longrightarrow> (P \<^sub>wf)\<^sup>t) \<and> stop_post))"
+    (RA \<circ> A) (true \<turnstile> (((\<not> (P \<^sub>wf)\<^sup>f) \<longrightarrow> (P \<^sub>wf)\<^sup>t) \<and> stop_post))"
 proof -
   let ?F = "(P \<^sub>wf)\<^sup>f"
   let ?T = "(P \<^sub>wf)\<^sup>t"
@@ -374,12 +560,10 @@ qed
 
 subsection \<open>Skip\<close>
 
-(* \<exists> y \<in> ac' \<bullet> \<not> y.wait \<and> y.tr = s.tr *)
+(* Paper Definition 42: \<in>\<^sub>a\<^sub>c y \<bullet> \<not> y.wait \<and> y.tr = s.tr *)
 definition skip_post :: "'e reactive_angelic_design" where
-[pred]: "skip_post = (\<lambda> (x, y).
-  \<exists> z \<in> achoices.ac\<^sub>v (des_vars.more y).
-    \<not> rad_state.wait\<^sub>v z \<and>
-    rad_state.tr\<^sub>v z = rad_state.tr\<^sub>v (astate.s\<^sub>v (des_vars.more x)))"
+[pred]: "skip_post = (\<in>\<^sub>a\<^sub>c y. (\<lambda> (s0, ac1).
+  \<not> rad_state.wait\<^sub>v y \<and> rad_state.tr\<^sub>v y = rad_state.tr\<^sub>v (astate.s\<^sub>v (des_vars.more s0))))"
 
 (* Paper Definition 42. *)
 definition Skip_RAD :: "'e reactive_angelic_design" ("Skip\<^sub>R\<^sub>A\<^sub>D") where
@@ -389,7 +573,7 @@ definition Skip_RAD :: "'e reactive_angelic_design" ("Skip\<^sub>R\<^sub>A\<^sub
 lemma skip_post_p2ac:
   "skip_post = p2ac \<lceil>(\<lambda> (s, y).
     \<not> rad_state.wait\<^sub>v y \<and> rad_state.tr\<^sub>v y = rad_state.tr\<^sub>v s)\<rceil>\<^sub>D"
-  by (simp add: skip_post_def p2ac_def fun_eq_iff subst_app_def
+  by (simp add: skip_post_def ades_singleton_choice_def p2ac_def fun_eq_iff subst_app_def
       subst_ext_def SEXP_def lens_defs des_vars.more\<^sub>L_def;
       pred_auto; blast)
 
@@ -397,12 +581,23 @@ lemma skip_post_PBMH [simp]: "PBMH_ades skip_post = skip_post"
   by (simp only: skip_post_p2ac PBMH_ades_p2ac)
 
 lemma rad_wait_false_skip_post: "(skip_post \<^sub>wf) = skip_post"
-  by (simp add: skip_post_def rad_wait_false_def fun_eq_iff subst_app_def
+  by (simp add: skip_post_def ades_singleton_choice_def rad_wait_false_def fun_eq_iff subst_app_def
       subst_upd_def subst_id_def SEXP_def lens_defs
       rad_state.wait_def astate.s_def des_vars.more\<^sub>L_def)
 
+lemma RA2_skip_post: "RA2 skip_post = skip_post"
+  by (simp add: RA2_def skip_post_def ades_singleton_choice_def rad_normalise_choices_def
+      rad_trace_difference_def rad_zero_trace_def fun_eq_iff Let_def;
+      pred_auto; force)
+
+lemma skip_post_unrest_ok_in [unrest]: "$ok\<^sup>< \<sharp> skip_post"
+  apply (simp add: unrest_lens skip_post_def ades_singleton_choice_def)
+  apply (simp add: subst_app_def subst_upd_def subst_id_def
+      SEXP_def lens_defs alpha_defs)
+  done
+
 lemma skip_post_unrest_ok [unrest]: "$ok\<^sup>> \<sharp> skip_post"
-  apply (simp add: unrest_lens skip_post_def)
+  apply (simp add: unrest_lens skip_post_def ades_singleton_choice_def)
   apply (simp add: subst_app_def subst_upd_def subst_id_def
       SEXP_def lens_defs alpha_defs)
   done
@@ -420,8 +615,7 @@ lemma Skip_RAD_is_RAD [closure]: "Skip\<^sub>R\<^sub>A\<^sub>D is RAD"
 theorem Skip_RAD_angelic_choice:
   assumes "P is RAD"
   shows "Skip\<^sub>R\<^sub>A\<^sub>D \<squnion>\<^sub>R\<^sub>A\<^sub>D P =
-    (RA \<circ> A) (true \<turnstile>
-      (skip_post \<and> ((\<not> (P \<^sub>wf)\<^sup>f) \<longrightarrow> (P \<^sub>wf)\<^sup>t)))"
+    (RA \<circ> A) (true \<turnstile> (skip_post \<and> ((\<not> (P \<^sub>wf)\<^sup>f) \<longrightarrow> (P \<^sub>wf)\<^sup>t)))"
 proof -
   let ?F = "(P \<^sub>wf)\<^sup>f"
   let ?T = "(P \<^sub>wf)\<^sup>t"
@@ -441,6 +635,326 @@ proof -
     apply (rule arg_cong[where f="RA \<circ> A"])
     apply (simp only: design_inf)
     by pred_auto
+  finally show ?thesis .
+qed
+
+subsection \<open>Sequential Composition\<close>
+
+text \<open>
+  Paper Section 6.4.7: sequential composition of reactive angelic designs
+  is exactly \<open>;;\<^sub>D\<^sub>A\<close> from the theory of angelic designs.  Its
+  paper Theorem 30 normal form and RAD closure law are proved in
+  \<open>utp_rad_seq\<close>.
+\<close>
+
+abbreviation seq_RAD ::
+  "'e reactive_angelic_design \<Rightarrow> 'e reactive_angelic_design \<Rightarrow>
+   'e reactive_angelic_design" (infixl ";;\<^sub>R\<^sub>A\<^sub>D" 75)
+where "P ;;\<^sub>R\<^sub>A\<^sub>D Q \<equiv> P ;;\<^sub>D\<^sub>A Q"
+
+(* Thesis Theorem T.4.5.15. *)
+lemma RAD_seq_demonic_distrib:
+  "(P \<sqinter>\<^sub>R\<^sub>A\<^sub>D Q) ;;\<^sub>R\<^sub>A\<^sub>D R = (P ;;\<^sub>R\<^sub>A\<^sub>D R) \<sqinter>\<^sub>R\<^sub>A\<^sub>D (Q ;;\<^sub>R\<^sub>A\<^sub>D R)"
+  by (rule angelic_design_seq_demonic)
+
+(* The observation repackaging distributes over sequential composition. *)
+lemma csp2rad_rel_seq_distrib:
+  fixes P Q :: "('e list, 'e set) rp_hrel"
+  shows "csp2rad_rel (P ;; Q) = (csp2rad_rel P ;; csp2rad_rel Q)"
+proof (rule ext)
+  fix w :: "'e rad_state des_vars_scheme \<times> 'e rad_state des_vars_scheme"
+  obtain x y where [simp]: "w = (x, y)" by (cases w) auto
+  have L: "csp2rad_rel (P ;; Q) w \<longleftrightarrow>
+      (\<exists>m. P (rad2csp_obs x, m) \<and> Q (m, rad2csp_obs y))"
+    by (simp add: csp2rad_rel_def; pred_auto)
+  have R: "(csp2rad_rel P ;; csp2rad_rel Q) w \<longleftrightarrow>
+      (\<exists>m. P (rad2csp_obs x, rad2csp_obs m) \<and>
+        Q (rad2csp_obs m, rad2csp_obs y))"
+    by (simp add: csp2rad_rel_def; pred_auto)
+  show "csp2rad_rel (P ;; Q) w = (csp2rad_rel P ;; csp2rad_rel Q) w"
+  proof (simp only: L R, rule iffI)
+    assume "\<exists>m. P (rad2csp_obs x, m) \<and> Q (m, rad2csp_obs y)"
+    then obtain m where "P (rad2csp_obs x, m)" and "Q (m, rad2csp_obs y)"
+      by blast
+    then show "\<exists>m. P (rad2csp_obs x, rad2csp_obs m) \<and>
+        Q (rad2csp_obs m, rad2csp_obs y)"
+      by (intro exI[where x="csp2rad_obs m"]) simp
+  next
+    assume "\<exists>m. P (rad2csp_obs x, rad2csp_obs m) \<and>
+        Q (rad2csp_obs m, rad2csp_obs y)"
+    then show "\<exists>m. P (rad2csp_obs x, m) \<and> Q (m, rad2csp_obs y)"
+      by blast
+  qed
+qed
+
+(* Thesis Theorem T.G.7.11, lifted to the reactive angelic mapping. *)
+lemma rad_p2ac_seq:
+  "rad_p2ac (P ;; Q) = (rad_p2ac P ;;\<^sub>R\<^sub>A\<^sub>D rad_p2ac Q)"
+  by (simp only: rad_p2ac_def comp_apply csp2rad_rel_seq_distrib
+      p2ac_seq)
+
+(* Thesis Theorem T.5.4.24: the correspondence of sequential composition with CSP. *)
+lemma RAD_seq_CSP_inverse:
+  "rad_ac2p (rad_p2ac P ;;\<^sub>R\<^sub>A\<^sub>D rad_p2ac Q) = P ;; Q"
+  by (simp only: rad_p2ac_seq[symmetric] rad_ac2p_p2ac_inverse')
+
+subsection \<open>Prefixing\<close>
+
+(* \<exists> y \<in> ac' \<bullet> (y.tr = s.tr \<and> a \<notin> y.ref) \<triangleleft> y.wait \<triangleright> y.tr = s.tr @ [a] *)
+definition prefix_post :: "'e \<Rightarrow> 'e reactive_angelic_design" where
+[pred]: "prefix_post a = (\<lambda> (s0, ac').
+  \<exists> y \<in> achoices.ac\<^sub>v (des_vars.more ac'). (((\<lambda> z. rad_state.tr\<^sub>v z =
+          rad_state.tr\<^sub>v (astate.s\<^sub>v (des_vars.more s0)) \<and>
+        a \<notin> rad_state.ref\<^sub>v z)
+      \<triangleleft> $rad_state.wait \<triangleright>
+      (\<lambda> z. rad_state.tr\<^sub>v z = rad_state.tr\<^sub>v (astate.s\<^sub>v (des_vars.more s0)) @ [a])) y))"
+
+(* Paper Definition 43 / Thesis Definition 124. *)
+definition PrefixSkip_RAD :: "'e \<Rightarrow> 'e reactive_angelic_design" where
+[pred]: "PrefixSkip_RAD a = (RA \<circ> A) (true \<turnstile> prefix_post a)"
+
+(* The paper's final-state quantifier is the predicate mapping p2ac. *)
+lemma prefix_post_p2ac:
+  "prefix_post a = p2ac \<lceil>(\<lambda> (s, y).
+    if rad_state.wait\<^sub>v y
+    then rad_state.tr\<^sub>v y = rad_state.tr\<^sub>v s \<and>
+      a \<notin> rad_state.ref\<^sub>v y
+    else rad_state.tr\<^sub>v y = rad_state.tr\<^sub>v s @ [a])\<rceil>\<^sub>D"
+  by (simp add: prefix_post_def expr_if_def rad_state.wait_def
+      p2ac_def fun_eq_iff subst_app_def
+      subst_ext_def SEXP_def lens_defs des_vars.more\<^sub>L_def;
+      pred_auto; blast)
+
+lemma prefix_post_PBMH [simp]:
+  "PBMH_ades (prefix_post a) = prefix_post a"
+  by (simp only: prefix_post_p2ac PBMH_ades_p2ac)
+
+lemma rad_wait_false_prefix_post:
+  "((prefix_post a) \<^sub>wf) = prefix_post a"
+  by (simp add: prefix_post_def expr_if_def rad_state.wait_def
+      rad_wait_false_def fun_eq_iff
+      subst_app_def subst_upd_def subst_id_def SEXP_def lens_defs
+      rad_state.wait_def astate.s_def des_vars.more\<^sub>L_def)
+
+lemma prefix_post_unrest_ok [unrest]: "$ok\<^sup>> \<sharp> prefix_post a"
+  apply (simp add: unrest_lens prefix_post_def expr_if_def
+      rad_state.wait_def)
+  apply (simp add: subst_app_def subst_upd_def subst_id_def
+      SEXP_def lens_defs alpha_defs)
+  done
+
+lemma prefix_design_is_H [closure]:
+  "(true \<turnstile> prefix_post a) is \<^bold>H"
+  by (rule design_is_H1_H2; simp add: unrest)
+
+lemma PrefixSkip_RAD_is_RAD [closure]: "PrefixSkip_RAD a is RAD"
+  unfolding PrefixSkip_RAD_def
+  apply (rule RAD_design_closure)
+   apply (rule prefix_design_is_H)
+  by (simp add: rad_wait_false_distrib rad_wait_false_prefix_post)
+
+(* Prefixing with the A absorbed into RA. *)
+lemma PrefixSkip_RAD_RA:
+  "PrefixSkip_RAD a = RA (true \<turnstile> prefix_post a)"
+  unfolding PrefixSkip_RAD_def
+  by (rule RA_A_absorb_design_true; simp add: Healthy_def' unrest)
+
+(* Paper Theorem 31 / Thesis Theorem T.5.4.26. *)
+theorem PrefixSkip_RAD_angelic_choice:
+  assumes "P is RAD"
+  shows "PrefixSkip_RAD a \<squnion>\<^sub>R\<^sub>A\<^sub>D P =
+    (RA \<circ> A) (true \<turnstile> (((\<not> (P \<^sub>wf)\<^sup>f) \<longrightarrow> (P \<^sub>wf)\<^sup>t) \<and> prefix_post a))"
+proof -
+  let ?F = "(P \<^sub>wf)\<^sup>f"
+  let ?T = "(P \<^sub>wf)\<^sup>t"
+  let ?DP = "(\<not> ?F) \<turnstile> ?T"
+  have "PrefixSkip_RAD a \<squnion>\<^sub>R\<^sub>A\<^sub>D P =
+      (RA \<circ> A) (true \<turnstile> prefix_post a) \<squnion> (RA \<circ> A) ?DP"
+    by (simp only: PrefixSkip_RAD_def
+        RAD_design_form'[OF assms, symmetric])
+  also have "... = (RA \<circ> A) ((true \<turnstile> prefix_post a) \<squnion> ?DP)"
+    apply (rule RA_A_angelic_choice)
+       apply (simp add: Healthy_def' design_as_disj PBMH_ades_disj
+          PBMH_ades_conj_ok)
+      apply (rule RAD_design_PBMH[OF assms])
+     apply (rule prefix_design_is_H)
+    by (rule rad_wait_false_design_is_H)
+  also have "... = (RA \<circ> A)
+      (true \<turnstile> (((\<not> ?F) \<longrightarrow> ?T) \<and> prefix_post a))"
+    apply (rule arg_cong[where f="RA \<circ> A"])
+    apply (simp only: design_inf)
+    by pred_auto
+  finally show ?thesis .
+qed
+
+(* Thesis Section 5.4.8: the compound process a \<rightarrow>\<^sub>R\<^sub>A\<^sub>D P
+   abbreviates (a \<rightarrow>\<^sub>R\<^sub>A\<^sub>D Skip\<^sub>R\<^sub>A\<^sub>D) ;;\<^sub>R\<^sub>A\<^sub>D P.  Its
+   Theorem T.5.4.29 normal form is future work; RAD closure is proved
+   in \<open>utp_rad_seq\<close>. *)
+definition Prefix_RAD ::
+  "'e \<Rightarrow> 'e reactive_angelic_design \<Rightarrow> 'e reactive_angelic_design"
+  (infixr "\<rightarrow>\<^sub>R\<^sub>A\<^sub>D" 80) where
+[pred]: "Prefix_RAD a P = (PrefixSkip_RAD a ;;\<^sub>R\<^sub>A\<^sub>D P)"
+
+subsection \<open>External Choice\<close>
+
+(*  \<exists> y \<in> ac' \<bullet>
+    (P \<and> Q)[{y}/ac'] \<triangleleft> y.tr = s.tr \<and> y.wait \<triangleright>
+    (P \<or> Q)[{y}/ac'] *)
+definition extchoice_post ::
+  "'e reactive_angelic_design \<Rightarrow> 'e reactive_angelic_design \<Rightarrow>
+   'e reactive_angelic_design" where
+[pred]: "extchoice_post P Q = (\<in>\<^sub>a\<^sub>c y. (\<lambda> (s0, ac1).
+  (((\<lambda> z. P (s0, ac1) \<and> Q (s0, ac1))
+    \<triangleleft> $rad_state.tr = \<guillemotleft>rad_state.tr\<^sub>v (astate.s\<^sub>v (des_vars.more s0))\<guillemotright> \<and>
+       $rad_state.wait \<triangleright>
+    (\<lambda> z. P (s0, ac1) \<or> Q (s0, ac1))) y)))"
+
+lemma rad_wait_false_extchoice_post:
+  "((extchoice_post P Q) \<^sub>wf) =
+   extchoice_post (P \<^sub>wf) (Q \<^sub>wf)"
+  by (simp add: extchoice_post_def ades_singleton_choice_def expr_if_def rad_state.wait_def
+      rad_state.tr_def SEXP_def rad_wait_false_def fun_eq_iff
+      subst_app_def subst_upd_def subst_id_def SEXP_def lens_defs
+      rad_state.wait_def astate.s_def des_vars.more\<^sub>L_def Let_def)
+
+lemma extchoice_post_ok_in_subst:
+  "(extchoice_post P Q)\<lbrakk>\<guillemotleft>b\<guillemotright>/ok\<^sup><\<rbrakk> =
+   extchoice_post (P\<lbrakk>\<guillemotleft>b\<guillemotright>/ok\<^sup><\<rbrakk>) (Q\<lbrakk>\<guillemotleft>b\<guillemotright>/ok\<^sup><\<rbrakk>)"
+  by (simp add: extchoice_post_def ades_singleton_choice_def expr_if_def rad_state.wait_def
+      rad_state.tr_def SEXP_def fun_eq_iff subst_app_def
+      subst_upd_def subst_id_def SEXP_def lens_defs des_vars.ok_def
+      astate.s_def des_vars.more\<^sub>L_def des_more_ok_update_commute
+      Let_def; pred_auto)
+
+(* Paper Definition 44 / Thesis Definition 125. *)
+definition extchoice_RAD ::
+  "'e reactive_angelic_design \<Rightarrow> 'e reactive_angelic_design \<Rightarrow>
+   'e reactive_angelic_design" (infixl "\<box>\<^sub>R\<^sub>A\<^sub>D" 68) where
+[pred]: "P \<box>\<^sub>R\<^sub>A\<^sub>D Q = (RA \<circ> A)
+  (((\<not> (P \<^sub>wf)\<^sup>f) \<and> (\<not> (Q \<^sub>wf)\<^sup>f)) \<turnstile>
+   extchoice_post ((P \<^sub>wf)\<^sup>t) ((Q \<^sub>wf)\<^sup>t))"
+
+lemma extchoice_post_unrest_ok [unrest]:
+  assumes "$ok\<^sup>> \<sharp> P" "$ok\<^sup>> \<sharp> Q"
+  shows "$ok\<^sup>> \<sharp> extchoice_post P Q"
+proof -
+  have put_P:
+      "\<forall> s0 ac1 v. P (s0, ac1\<lparr>des_vars.ok\<^sub>v := v\<rparr>) = P (s0, ac1)"
+    using assms(1)
+    apply (subst (asm) unrest_lens)
+     apply simp
+    by (simp add: lens_defs des_vars.ok_def case_prod_beta
+        split_paired_All)
+  have put_Q:
+      "\<forall> s0 ac1 v. Q (s0, ac1\<lparr>des_vars.ok\<^sub>v := v\<rparr>) = Q (s0, ac1)"
+    using assms(2)
+    apply (subst (asm) unrest_lens)
+     apply simp
+    by (simp add: lens_defs des_vars.ok_def case_prod_beta
+        split_paired_All)
+  show ?thesis
+    apply (subst unrest_lens)
+     apply simp
+    apply (simp add: extchoice_post_def ades_singleton_choice_def expr_if_def rad_state.wait_def
+      rad_state.tr_def SEXP_def Let_def lens_defs
+        des_vars.ok_def case_prod_beta)
+    using put_P put_Q
+    by (simp add: des_more_ok_update_commute)
+qed
+
+lemma extchoice_RAD_closure [closure]:
+  assumes "P is RAD" "Q is RAD"
+  shows "P \<box>\<^sub>R\<^sub>A\<^sub>D Q is RAD"
+  unfolding extchoice_RAD_def
+  apply (rule RAD_design_closure)
+   apply (rule design_is_H1_H2; simp add: unrest)
+  by (simp add: rad_wait_false_distrib rad_wait_false_extchoice_post)
+
+(* Composition with the Stop postcondition reduces both branches to
+   the bare singleton choice: the waiting branch of Stop holds exactly
+   on the states admitted by the conditional's guard. *)
+lemma extchoice_post_stop:
+  "extchoice_post X (RA2 (RA1 stop_post)) = \<in>\<^sub>a\<^sub>c(X)"
+  apply (simp only: RA1_RA2_commute'[symmetric] RA2_stop_post)
+  apply (simp add: extchoice_post_def ades_singleton_choice_def expr_if_def rad_state.wait_def
+      rad_state.tr_def SEXP_def ades_singleton_choice_def
+      RA1_def stop_post_def rad_trace_extensions_def fun_eq_iff
+      Let_def lens_defs rad_state.wait_def astate.s_def
+      des_vars.more\<^sub>L_def)
+  by (pred_auto; blast)
+
+(* Paper Theorem 32 / Thesis Theorem T.5.4.30: external choice with
+   Stop collapses the angelic nondeterminism of P. *)
+theorem extchoice_RAD_Stop:
+  assumes "P is RAD"
+  shows "P \<box>\<^sub>R\<^sub>A\<^sub>D Stop\<^sub>R\<^sub>A\<^sub>D =
+    (RA \<circ> A) ((\<not> (P \<^sub>wf)\<^sup>f) \<turnstile>
+      \<in>\<^sub>a\<^sub>c((P \<^sub>wf)\<^sup>t))"
+proof -
+  let ?F = "(P \<^sub>wf)\<^sup>f" and ?T = "(P \<^sub>wf)\<^sup>t"
+  let ?SF = "(Stop\<^sub>R\<^sub>A\<^sub>D \<^sub>wf)\<^sup>f"
+  let ?ST = "(Stop\<^sub>R\<^sub>A\<^sub>D \<^sub>wf)\<^sup>t"
+  have pre_push:
+      "((\<not> ?F) \<and> (\<not> ?SF))\<lbrakk>True/ok\<^sup><\<rbrakk> =
+       (\<not> ?F)\<lbrakk>True/ok\<^sup><\<rbrakk>"
+    by (simp add: usubst
+        Stop_RAD_wf_ok_false_subst[simplified usubst]; pred_auto)
+  have post_push:
+      "(extchoice_post ?T ?ST)\<lbrakk>True/ok\<^sup><\<rbrakk> =
+       (\<in>\<^sub>a\<^sub>c(?T))\<lbrakk>True/ok\<^sup><\<rbrakk>"
+    by (simp only: extchoice_post_ok_in_subst
+        ades_singleton_choice_ok_in_subst
+        Stop_RAD_wf_ok_true_subst extchoice_post_stop)
+  have "(((\<not> ?F) \<and> (\<not> ?SF)) \<turnstile> extchoice_post ?T ?ST) =
+        ((\<not> ?F) \<turnstile> \<in>\<^sub>a\<^sub>c(?T))"
+    using arg_cong2[where f=design, OF pre_push post_push]
+    by (simp only: design_subst_ok)
+  then show ?thesis
+    by (simp only: extchoice_RAD_def)
+qed
+
+(* Theorem 32 in the paper's raw format:
+   \<exists> y \<bullet> (P\<^sup>t\<^sub>f)[{y}/ac'] \<and> y \<in> ac' *)
+lemma extchoice_RAD_Stop_expanded:
+  assumes "P is RAD"
+  shows "P \<box>\<^sub>R\<^sub>A\<^sub>D Stop\<^sub>R\<^sub>A\<^sub>D =
+    (RA \<circ> A) ((\<not> (P \<^sub>wf)\<^sup>f) \<turnstile>
+      (\<lambda> (s0, ac'). \<exists> y \<in> achoices.ac\<^sub>v (des_vars.more ac').
+          ((P \<^sub>wf)\<^sup>t) (s0, des_vars.more_update
+              (achoices.ac\<^sub>v_update (\<lambda>_. {y})) ac')))"
+  by (simp only: extchoice_RAD_Stop[OF assms]
+      ades_singleton_choice_def)
+
+(* Paper Theorem 33 / Thesis Theorem T.5.4.31 *)
+theorem extchoice_RAD_Stop_unit:
+  assumes "P is RAD" "P is A2"
+  shows "P \<box>\<^sub>R\<^sub>A\<^sub>D Stop\<^sub>R\<^sub>A\<^sub>D = P"
+proof -
+  let ?F = "(P \<^sub>wf)\<^sup>f" and ?T = "(P \<^sub>wf)\<^sup>t"
+  have not_F_PBMH: "(\<not> (\<not> ?F)) is PBMH_ades"
+    by (simp only: pred_ba.double_compl
+        RAD_wf_ok_false_PBMH[OF assms(1)])
+  have unrests: "$ok\<^sup>> \<sharp> (\<not> ?F)" "$ok\<^sup>> \<sharp> ?T"
+    by (simp_all add: unrest)
+  have RA1_eq: "RA1 (\<in>\<^sub>a\<^sub>c(?T)) = RA1 ?T"
+    by (rule RA1_singleton_absorb[OF RAD_wf_ok_true_PBMH[OF assms(1)]
+        A2_wf_ok_true_singleton_reduce[OF assms(2)]])
+  have "P \<box>\<^sub>R\<^sub>A\<^sub>D Stop\<^sub>R\<^sub>A\<^sub>D =
+      (RA \<circ> A) ((\<not> ?F) \<turnstile> \<in>\<^sub>a\<^sub>c(?T))"
+    by (rule extchoice_RAD_Stop[OF assms(1)])
+  also have "... = RA ((\<not> ?F) \<turnstile> \<in>\<^sub>a\<^sub>c(?T))"
+    by (rule RA_A_absorb_design[OF not_F_PBMH _ unrests(1)])
+      (simp_all add: Healthy_def' unrest unrests)
+  also have "... =
+      RA ((\<not> ?F) \<turnstile> (RA2 \<circ> RA1) (\<in>\<^sub>a\<^sub>c(?T)))"
+    by (rule RA_design_post)
+  also have "... = RA ((\<not> ?F) \<turnstile> (RA2 \<circ> RA1) ?T)"
+    by (simp only: comp_apply RA1_eq)
+  also have "... = RA ((\<not> ?F) \<turnstile> ?T)"
+    by (rule RA_design_post[symmetric])
+  also have "... = P"
+    by (rule RAD_RA_design_form[OF assms(1), symmetric])
   finally show ?thesis .
 qed
 
