utp_rad_examples.thy
@@ -1,0 +1,553 @@
+section \<open>Reactive Angelic Design Examples\<close>
+
+text \<open>
+  The worked examples of the paper's Section 6.4 (Examples 15--17 and
+  Lemmas 8--9), collected apart from the operator theories.
+\<close>
+
+theory utp_rad_examples
+  imports utp_rad_seq
+begin
+
+subsection \<open>Angelic choice of Stop and Skip (Example 15, Lemma 8)\<close>
+
+(* Paper Example 15 / Thesis Example 32: the angelic choice between
+   deadlock and termination is not resolved in favour of either. *)
+lemma Stop_Skip_angelic_choice:
+  "Stop\<^sub>R\<^sub>A\<^sub>D \<squnion>\<^sub>R\<^sub>A\<^sub>D Skip\<^sub>R\<^sub>A\<^sub>D =
+   (RA \<circ> A) (true \<turnstile> (stop_post \<and> skip_post))"
+proof -
+  have "Stop\<^sub>R\<^sub>A\<^sub>D \<squnion>\<^sub>R\<^sub>A\<^sub>D Skip\<^sub>R\<^sub>A\<^sub>D =
+      (RA \<circ> A) ((true \<turnstile> stop_post) \<squnion> (true \<turnstile> skip_post))"
+    unfolding Stop_RAD_def Skip_RAD_def
+    apply (rule RA_A_angelic_choice)
+       apply (simp add: Healthy_def' design_as_disj PBMH_ades_disj
+          PBMH_ades_conj_ok)
+      apply (simp add: Healthy_def' design_as_disj PBMH_ades_disj
+          PBMH_ades_conj_ok)
+     apply (rule stop_design_is_H)
+    by (rule skip_design_is_H)
+  also have "... = (RA \<circ> A) (true \<turnstile> (stop_post \<and> skip_post))"
+    apply (rule arg_cong[where f="RA \<circ> A"])
+    apply (simp only: design_inf)
+    by pred_auto
+  finally show ?thesis .
+qed
+
+(* Example 15 with the A absorbed into RA. *)
+lemma Stop_Skip_angelic_choice_RA:
+  "Stop\<^sub>R\<^sub>A\<^sub>D \<squnion>\<^sub>R\<^sub>A\<^sub>D Skip\<^sub>R\<^sub>A\<^sub>D =
+   RA (true \<turnstile> (stop_post \<and> skip_post))"
+  unfolding Stop_Skip_angelic_choice
+  by (rule RA_A_absorb_design_true;
+      (rule PBMH_ades_conj_closure)?;
+      simp add: Healthy_def' unrest)
+
+(* Under the singleton angelic choice imposed by ac2p, a final state
+   cannot both wait and terminate. *)
+lemma rad_ac2p_stop_skip_design:
+  "rad_ac2p (true \<turnstile> (stop_post \<and> skip_post)) = (true \<turnstile> false)"
+  by (simp add: rad_ac2p_def; pred_auto; blast)
+
+abbreviation top_R ("\<top>\<^sub>R") where "\<top>\<^sub>R \<equiv> \<^bold>R (true \<turnstile> false)"
+
+(* Paper Lemma 8 / Thesis Lemma L.5.4.2: mapping the choice between
+   deadlock and termination into CSP yields the top of the reactive
+   design lattice. *)
+lemma rad_ac2p_Stop_Skip:
+  "rad_ac2p (Stop\<^sub>R\<^sub>A\<^sub>D \<squnion>\<^sub>R\<^sub>A\<^sub>D Skip\<^sub>R\<^sub>A\<^sub>D) = \<top>\<^sub>R"
+proof -
+  have SS_PBMH: "(stop_post \<and> skip_post) is PBMH_ades"
+    by (rule PBMH_ades_conj_closure; simp add: Healthy_def')
+  have D_PBMH: "(true \<turnstile> (stop_post \<and> skip_post)) is PBMH_ades"
+    unfolding Healthy_def'
+    by (simp add: design_as_disj PBMH_ades_disj PBMH_ades_conj_ok
+        SS_PBMH[unfolded Healthy_def'])
+  have D_H: "(true \<turnstile> (stop_post \<and> skip_post)) is \<^bold>H"
+    by (rule design_is_H1_H2; simp add: unrest)
+  have "rad_ac2p (Stop\<^sub>R\<^sub>A\<^sub>D \<squnion>\<^sub>R\<^sub>A\<^sub>D Skip\<^sub>R\<^sub>A\<^sub>D) =
+      rad_ac2p (RA (true \<turnstile> (stop_post \<and> skip_post)))"
+    by (simp only: Stop_Skip_angelic_choice
+        RA_A_absorb[OF D_PBMH D_H])
+  also have "... = \<^bold>R (rad_ac2p (true \<turnstile> (stop_post \<and> skip_post)))"
+    by (rule rad_ac2p_RA[OF D_PBMH, simplified comp_apply])
+  also have "... = \<^bold>R (true \<turnstile> false)"
+    by (simp only: rad_ac2p_stop_skip_design)
+  finally show ?thesis .
+qed
+
+subsection \<open>Avoiding divergence after termination (Lemma 9)\<close>
+
+(* Paper Lemma 9 / Thesis Lemma L.5.4.3: the angel avoids the
+   terminating branch, since its handover to Chaos would diverge. *)
+lemma Stop_Skip_seq_Chaos:
+  "(Stop\<^sub>R\<^sub>A\<^sub>D \<squnion>\<^sub>R\<^sub>A\<^sub>D Skip\<^sub>R\<^sub>A\<^sub>D) ;;\<^sub>R\<^sub>A\<^sub>D Chaos\<^sub>R\<^sub>A\<^sub>D = Stop\<^sub>R\<^sub>A\<^sub>D"
+proof -
+  let ?J = "stop_post \<and> skip_post"
+  have J_PBMH: "?J is PBMH_ades"
+    by (rule PBMH_ades_conj_closure; simp add: Healthy_def')
+  have not_true_PBMH:
+      "(\<not> (true :: 'e reactive_angelic_design)) is PBMH_ades"
+    by (simp only: pred_ba.compl_top_eq false_PBMH_ades)
+  have component_unrests:
+      "$ok\<^sup>> \<sharp> (true :: 'e reactive_angelic_design)"
+      "$ok\<^sup>> \<sharp> ?J"
+      "$ok\<^sup>< \<sharp> (false :: 'e reactive_angelic_design)"
+      "$ok\<^sup>< \<sharp> (true :: 'e reactive_angelic_design)"
+    by (simp_all add: unrest)
+  have handover_false:
+      "(RA1 ?J ;;\<^sub>A\<^sub>D
+        ((\<not> rad_wait_lens\<^sup><) \<and> RA2 (RA1 true))) = false"
+    by (simp add: RA1_def aseq_ades_def stop_post_def skip_post_def ades_singleton_choice_def
+        fun_eq_iff Let_def; pred_auto; auto)
+  have continuation_stop:
+      "(RA1 ?J ;;\<^sub>A\<^sub>D
+        (ades_state_choice \<triangleleft> $rad_wait_lens\<^sup>< \<triangleright>
+          RA2 (RA1 true))) = stop_post"
+    apply (simp only: RA1_RA2_commute'[symmetric] RA2_true)
+    apply (simp add: RA1_def aseq_ades_def stop_post_def
+        skip_post_def ades_singleton_choice_def ades_state_choice_def expr_if_def
+        rad_trace_extensions_def fun_eq_iff Let_def)
+    apply clarify
+    subgoal for a b
+      by (cases "astate.s\<^sub>v (des_vars.more a)";
+          cases "des_vars.more a"; cases a;
+          cases "des_vars.more b"; cases b;
+          auto simp add: lens_defs des_vars.ok_def rad_state.wait_def
+            astate.s_def des_vars.more\<^sub>L_def conj_pred_def true_pred_def
+            intro: order_trans;
+          rule_tac x="rad_state.wait\<^sub>v_update (\<lambda>_. False) y"
+            in bexI;
+          auto)
+    done
+  have seq_form:
+      "(RA (true \<turnstile> ?J) ;;\<^sub>D\<^sub>A RA true) =
+       RA (true \<turnstile> stop_post)"
+    using RA_design_seq[
+      where P=true and Q="?J" and R=false and S=true,
+      OF component_unrests not_true_PBMH J_PBMH]
+    by (simp only: design_false_pre pred_ba.compl_top_eq
+        pred_ba.compl_bot_eq pred_impl_laws pred_ba.inf_idem
+        RA1_false aseq_ades_false_left handover_false
+        continuation_stop)
+  show ?thesis
+    by (subst Stop_Skip_angelic_choice_RA;
+        simp only: Chaos_RAD_RA seq_form Stop_RAD_RA)
+qed
+
+subsection \<open>Prefixed deadlock avoids divergence (Example 16)\<close>
+
+(* Postcondition of a \<rightarrow>\<^sub>R\<^sub>A\<^sub>D Stop\<^sub>R\<^sub>A\<^sub>D: either the
+   event has not yet happened and is offered, or it has happened and
+   the process deadlocks. *)
+definition prefix_stop_post :: "'e \<Rightarrow> 'e reactive_angelic_design" where
+[pred]: "prefix_stop_post a = (\<lambda> (s0, ac').
+  \<exists> y \<in> achoices.ac\<^sub>v (des_vars.more ac').
+    rad_state.wait\<^sub>v y \<and>
+    (rad_state.tr\<^sub>v y =
+       rad_state.tr\<^sub>v (astate.s\<^sub>v (des_vars.more s0)) \<and>
+     a \<notin> rad_state.ref\<^sub>v y \<or>
+     rad_state.tr\<^sub>v y =
+       rad_state.tr\<^sub>v (astate.s\<^sub>v (des_vars.more s0)) @ [a]))"
+
+(* The paper's final-state quantifier is the predicate mapping p2ac. *)
+lemma prefix_stop_post_p2ac:
+  "prefix_stop_post a = p2ac \<lceil>(\<lambda> (s, y).
+    rad_state.wait\<^sub>v y \<and>
+    (rad_state.tr\<^sub>v y = rad_state.tr\<^sub>v s \<and>
+       a \<notin> rad_state.ref\<^sub>v y \<or>
+     rad_state.tr\<^sub>v y = rad_state.tr\<^sub>v s @ [a]))\<rceil>\<^sub>D"
+  by (simp add: prefix_stop_post_def p2ac_def fun_eq_iff subst_app_def
+      subst_ext_def SEXP_def lens_defs des_vars.more\<^sub>L_def;
+      pred_auto; blast)
+
+lemma prefix_stop_post_PBMH [simp]:
+  "PBMH_ades (prefix_stop_post a) = prefix_stop_post a"
+  by (simp only: prefix_stop_post_p2ac PBMH_ades_p2ac)
+
+lemma prefix_stop_post_unrest_ok [unrest]:
+  "$ok\<^sup>> \<sharp> prefix_stop_post a"
+  apply (simp add: unrest_lens prefix_stop_post_def)
+  apply (simp add: subst_app_def subst_upd_def subst_id_def
+      SEXP_def lens_defs alpha_defs)
+  done
+
+(* The continuation of prefixing into Stop: before the event the
+   process waits offering a; after it the handover state is a
+   deadlocked state whose trace records the event. *)
+lemma prefix_continuation_stop:
+  "(RA1 (prefix_post a) ;;\<^sub>A\<^sub>D
+    (ades_state_choice \<triangleleft> $rad_wait_lens\<^sup>< \<triangleright>
+      RA2 (RA1 stop_post))) = prefix_stop_post a"
+  apply (simp only: RA1_RA2_commute'[symmetric] RA2_stop_post)
+  apply (simp add: RA1_def aseq_ades_def prefix_post_def stop_post_def
+      prefix_stop_post_def ades_state_choice_def expr_if_def
+      rad_trace_extensions_def fun_eq_iff Let_def
+      lens_defs rad_state.wait_def astate.s_def des_vars.more\<^sub>L_def
+      bex_nonempty_absorb)
+  apply clarify
+  subgoal for x0 y0
+    apply (rule iffI)
+     apply fastforce
+    apply (elim bexE conjE disjE)
+     apply (rule_tac x=y in bexI; fastforce)
+    apply (rule_tac x="rad_state.wait\<^sub>v_update (\<lambda>_. False) y"
+        in bexI; fastforce)
+    done
+  done
+
+(* Thesis Theorem T.5.4.29 instantiated to Stop: the design form of
+   a \<rightarrow>\<^sub>R\<^sub>A\<^sub>D Stop\<^sub>R\<^sub>A\<^sub>D. *)
+lemma Prefix_Stop_RAD_RA:
+  "(a \<rightarrow>\<^sub>R\<^sub>A\<^sub>D Stop\<^sub>R\<^sub>A\<^sub>D) = RA (true \<turnstile> prefix_stop_post a)"
+proof -
+  have component_unrests:
+      "$ok\<^sup>> \<sharp> (true :: 'e reactive_angelic_design)"
+      "$ok\<^sup>> \<sharp> prefix_post a"
+      "$ok\<^sup>< \<sharp> (true :: 'e reactive_angelic_design)"
+      "$ok\<^sup>< \<sharp> stop_post"
+    by (simp_all add: unrest)
+  have not_true_PBMH:
+      "(\<not> (true :: 'e reactive_angelic_design)) is PBMH_ades"
+    by (simp only: pred_ba.compl_top_eq false_PBMH_ades)
+  have prefix_PBMH: "prefix_post a is PBMH_ades"
+    by (simp add: Healthy_def')
+  have "(a \<rightarrow>\<^sub>R\<^sub>A\<^sub>D Stop\<^sub>R\<^sub>A\<^sub>D) =
+      (RA (true \<turnstile> prefix_post a) ;;\<^sub>D\<^sub>A
+       RA (true \<turnstile> stop_post))"
+    by (simp only: Prefix_RAD_def PrefixSkip_RAD_RA Stop_RAD_RA)
+  also have "... = RA (true \<turnstile> prefix_stop_post a)"
+    using RA_design_seq[
+      where P=true and Q="prefix_post a" and R=true and S=stop_post,
+      OF component_unrests not_true_PBMH prefix_PBMH]
+    by (simp only: pred_ba.compl_top_eq pred_ba.compl_bot_eq
+        RA1_false RA2_false aseq_ades_false_left
+        pred_ba.inf_bot_right RA1_aseq_false pred_ba.inf_idem
+        pred_impl_laws prefix_continuation_stop)
+  finally show ?thesis .
+qed
+
+(* The angelic choice of a \<rightarrow>\<^sub>R\<^sub>A\<^sub>D Stop\<^sub>R\<^sub>A\<^sub>D and
+   Skip\<^sub>R\<^sub>A\<^sub>D, with the A absorbed into RA. *)
+lemma Prefix_Stop_Skip_angelic_choice_RA:
+  "(a \<rightarrow>\<^sub>R\<^sub>A\<^sub>D Stop\<^sub>R\<^sub>A\<^sub>D) \<squnion>\<^sub>R\<^sub>A\<^sub>D Skip\<^sub>R\<^sub>A\<^sub>D =
+   RA (true \<turnstile> (prefix_stop_post a \<and> skip_post))"
+proof -
+  have psp_absorb:
+      "(RA \<circ> A) (true \<turnstile> prefix_stop_post a) =
+       RA (true \<turnstile> prefix_stop_post a)"
+    by (rule RA_A_absorb_design_true; simp add: Healthy_def' unrest)
+  have conj_absorb:
+      "(RA \<circ> A) (true \<turnstile> (prefix_stop_post a \<and> skip_post)) =
+       RA (true \<turnstile> (prefix_stop_post a \<and> skip_post))"
+    by (rule RA_A_absorb_design_true;
+        (rule PBMH_ades_conj_closure)?;
+        simp add: Healthy_def' unrest)
+  have "(a \<rightarrow>\<^sub>R\<^sub>A\<^sub>D Stop\<^sub>R\<^sub>A\<^sub>D) \<squnion>\<^sub>R\<^sub>A\<^sub>D Skip\<^sub>R\<^sub>A\<^sub>D =
+      (RA \<circ> A) (true \<turnstile> prefix_stop_post a) \<squnion>
+      (RA \<circ> A) (true \<turnstile> skip_post)"
+    by (simp only: Prefix_Stop_RAD_RA psp_absorb Skip_RAD_def)
+  also have "... = (RA \<circ> A)
+      ((true \<turnstile> prefix_stop_post a) \<squnion> (true \<turnstile> skip_post))"
+    apply (rule RA_A_angelic_choice)
+       apply (simp add: Healthy_def' design_as_disj PBMH_ades_disj
+          PBMH_ades_conj_ok)
+      apply (simp add: Healthy_def' design_as_disj PBMH_ades_disj
+          PBMH_ades_conj_ok)
+     apply (rule design_is_H1_H2; simp add: unrest)
+    by (rule design_is_H1_H2; simp add: unrest)
+  also have "... = (RA \<circ> A)
+      (true \<turnstile> (prefix_stop_post a \<and> skip_post))"
+    apply (rule arg_cong[where f="RA \<circ> A"])
+    apply (simp only: design_inf)
+    by pred_auto
+  finally show ?thesis
+    by (simp only: conj_absorb)
+qed
+
+(* Paper Example 16 / Thesis Example 33: the angel avoids the
+   divergence following termination by choosing to perform a and
+   deadlock. *)
+lemma Prefix_Stop_Skip_seq_Chaos:
+  "((a \<rightarrow>\<^sub>R\<^sub>A\<^sub>D Stop\<^sub>R\<^sub>A\<^sub>D) \<squnion>\<^sub>R\<^sub>A\<^sub>D Skip\<^sub>R\<^sub>A\<^sub>D) ;;\<^sub>R\<^sub>A\<^sub>D
+   Chaos\<^sub>R\<^sub>A\<^sub>D = (a \<rightarrow>\<^sub>R\<^sub>A\<^sub>D Stop\<^sub>R\<^sub>A\<^sub>D)"
+proof -
+  let ?J = "prefix_stop_post a \<and> skip_post"
+  have J_PBMH: "?J is PBMH_ades"
+    by (rule PBMH_ades_conj_closure; simp add: Healthy_def')
+  have not_true_PBMH:
+      "(\<not> (true :: 'e reactive_angelic_design)) is PBMH_ades"
+    by (simp only: pred_ba.compl_top_eq false_PBMH_ades)
+  have component_unrests:
+      "$ok\<^sup>> \<sharp> (true :: 'e reactive_angelic_design)"
+      "$ok\<^sup>> \<sharp> ?J"
+      "$ok\<^sup>< \<sharp> (false :: 'e reactive_angelic_design)"
+      "$ok\<^sup>< \<sharp> (true :: 'e reactive_angelic_design)"
+    by (simp_all add: unrest)
+  have handover_false:
+      "(RA1 ?J ;;\<^sub>A\<^sub>D
+        ((\<not> rad_wait_lens\<^sup><) \<and> RA2 (RA1 true))) = false"
+    by (simp add: RA1_def aseq_ades_def prefix_stop_post_def
+        skip_post_def ades_singleton_choice_def fun_eq_iff Let_def; pred_auto; auto)
+  have continuation_prefix_stop:
+      "(RA1 ?J ;;\<^sub>A\<^sub>D
+        (ades_state_choice \<triangleleft> $rad_wait_lens\<^sup>< \<triangleright>
+          RA2 (RA1 true))) = prefix_stop_post a"
+    apply (simp only: RA1_RA2_commute'[symmetric] RA2_true)
+    apply (simp add: RA1_def aseq_ades_def prefix_stop_post_def
+        skip_post_def ades_singleton_choice_def ades_state_choice_def expr_if_def
+        rad_trace_extensions_def fun_eq_iff Let_def
+        lens_defs rad_state.wait_def astate.s_def des_vars.more\<^sub>L_def
+        conj_pred_def true_pred_def ex_in_conv[symmetric])
+    apply clarify
+    subgoal for x0 y0
+      apply (rule iffI)
+       apply fastforce
+      apply (elim bexE conjE)
+      apply (rule conjI)
+       apply (rule_tac x=y in bexI; fastforce)
+      apply (rule conjI)
+       apply (rule_tac x="rad_state.wait\<^sub>v_update (\<lambda>_. False)
+           (rad_state.tr\<^sub>v_update
+             (\<lambda>_. rad_state.tr\<^sub>v (astate.s\<^sub>v (des_vars.more x0)))
+             y)" in bexI)
+        apply fastforce
+       apply (rule IntI)
+        apply fastforce
+       apply (simp only: mem_Collect_eq)
+       apply (rule conjI)
+        apply fastforce
+       apply (rule impI)
+       apply (rule_tac x=y in exI)
+       apply fastforce
+      apply (rule_tac x=y in exI)
+      apply fastforce
+      done
+    done
+  have seq_form:
+      "(RA (true \<turnstile> ?J) ;;\<^sub>D\<^sub>A RA true) =
+       RA (true \<turnstile> prefix_stop_post a)"
+    using RA_design_seq[
+      where P=true and Q="?J" and R=false and S=true,
+      OF component_unrests not_true_PBMH J_PBMH]
+    by (simp only: design_false_pre pred_ba.compl_top_eq
+        pred_ba.compl_bot_eq pred_impl_laws pred_ba.inf_idem
+        RA1_false aseq_ades_false_left handover_false
+        continuation_prefix_stop)
+  show ?thesis
+    by (subst Prefix_Stop_Skip_angelic_choice_RA;
+        simp only: Chaos_RAD_RA seq_form Prefix_Stop_RAD_RA[symmetric])
+qed
+
+subsection \<open>Prefixed termination avoids divergence (Example 17)\<close>
+
+(* The failure observation of a \<rightarrow>\<^sub>R\<^sub>A\<^sub>D
+   Chaos\<^sub>R\<^sub>A\<^sub>D: the event has occurred. *)
+definition prefix_diverge_post :: "'e \<Rightarrow> 'e reactive_angelic_design"
+where
+[pred]: "prefix_diverge_post a = (\<lambda> (s0, ac').
+  \<exists> y \<in> achoices.ac\<^sub>v (des_vars.more ac').
+    rad_state.tr\<^sub>v (astate.s\<^sub>v (des_vars.more s0)) @ [a] \<le>
+    rad_state.tr\<^sub>v y)"
+
+(* The event is offered and has not yet occurred. *)
+definition prefix_offer_post :: "'e \<Rightarrow> 'e reactive_angelic_design"
+where
+[pred]: "prefix_offer_post a = (\<lambda> (s0, ac').
+  \<exists> y \<in> achoices.ac\<^sub>v (des_vars.more ac').
+    rad_state.wait\<^sub>v y \<and>
+    rad_state.tr\<^sub>v y =
+      rad_state.tr\<^sub>v (astate.s\<^sub>v (des_vars.more s0)) \<and>
+    a \<notin> rad_state.ref\<^sub>v y)"
+
+lemma prefix_diverge_post_p2ac:
+  "prefix_diverge_post a = p2ac \<lceil>(\<lambda> (s, y).
+    rad_state.tr\<^sub>v s @ [a] \<le> rad_state.tr\<^sub>v y)\<rceil>\<^sub>D"
+  by (simp add: prefix_diverge_post_def p2ac_def fun_eq_iff
+      subst_app_def subst_ext_def SEXP_def lens_defs
+      des_vars.more\<^sub>L_def; pred_auto; blast)
+
+lemma prefix_offer_post_p2ac:
+  "prefix_offer_post a = p2ac \<lceil>(\<lambda> (s, y).
+    rad_state.wait\<^sub>v y \<and> rad_state.tr\<^sub>v y = rad_state.tr\<^sub>v s \<and>
+    a \<notin> rad_state.ref\<^sub>v y)\<rceil>\<^sub>D"
+  by (simp add: prefix_offer_post_def p2ac_def fun_eq_iff
+      subst_app_def subst_ext_def SEXP_def lens_defs
+      des_vars.more\<^sub>L_def; pred_auto; blast)
+
+lemma prefix_diverge_post_PBMH [simp]:
+  "PBMH_ades (prefix_diverge_post a) = prefix_diverge_post a"
+  by (simp only: prefix_diverge_post_p2ac PBMH_ades_p2ac)
+
+lemma prefix_offer_post_PBMH [simp]:
+  "PBMH_ades (prefix_offer_post a) = prefix_offer_post a"
+  by (simp only: prefix_offer_post_p2ac PBMH_ades_p2ac)
+
+lemma prefix_diverge_post_unrest_ok [unrest]:
+  "$ok\<^sup>> \<sharp> prefix_diverge_post a"
+  apply (simp add: unrest_lens prefix_diverge_post_def)
+  apply (simp add: subst_app_def subst_upd_def subst_id_def
+      SEXP_def lens_defs alpha_defs)
+  done
+
+lemma prefix_offer_post_unrest_ok [unrest]:
+  "$ok\<^sup>> \<sharp> prefix_offer_post a"
+  apply (simp add: unrest_lens prefix_offer_post_def)
+  apply (simp add: subst_app_def subst_upd_def subst_id_def
+      SEXP_def lens_defs alpha_defs)
+  done
+
+(* Handing the prefix over to an arbitrary continuation records
+   exactly that the event has occurred. *)
+lemma prefix_handover_diverge:
+  "(RA1 (prefix_post a) ;;\<^sub>A\<^sub>D
+    ((\<not> rad_wait_lens\<^sup><) \<and> RA2 (RA1 true))) =
+   prefix_diverge_post a"
+  apply (simp only: RA1_RA2_commute'[symmetric] RA2_true)
+  apply (simp add: RA1_def aseq_ades_def prefix_post_def expr_if_def
+      rad_state.wait_def
+      prefix_diverge_post_def rad_trace_extensions_def fun_eq_iff
+      Let_def lens_defs rad_state.wait_def astate.s_def
+      des_vars.more\<^sub>L_def true_pred_def conj_pred_def
+      not_pred_def SEXP_def subst_ext_def
+      subst_app_def ex_in_conv[symmetric])
+  apply clarify
+  subgoal for x0 y0
+    apply (rule iffI)
+     apply (fastforce intro: order_trans)
+    apply (elim bexE)
+    subgoal for y
+      apply (rule conjI)
+       apply (rule_tac x="rad_state.wait\<^sub>v_update (\<lambda>_. False)
+           (rad_state.tr\<^sub>v_update
+             (\<lambda>_. rad_state.tr\<^sub>v (astate.s\<^sub>v (des_vars.more x0)) @ [a])
+             y)" in bexI; fastforce)
+      by (rule_tac x="rad_state.wait\<^sub>v_update (\<lambda>_. False)
+          (rad_state.tr\<^sub>v_update
+            (\<lambda>_. rad_state.tr\<^sub>v (astate.s\<^sub>v (des_vars.more x0)) @ [a])
+            y)" in exI; fastforce)
+    done
+  done
+
+(* The continuation of the prefix into Chaos: either the event is
+   still offered, or it has occurred and anything may follow. *)
+lemma prefix_continuation_chaos:
+  "(RA1 (prefix_post a) ;;\<^sub>A\<^sub>D
+    (ades_state_choice \<triangleleft> $rad_wait_lens\<^sup>< \<triangleright>
+      RA2 (RA1 true))) =
+   (prefix_offer_post a \<or> prefix_diverge_post a)"
+  apply (simp only: RA1_RA2_commute'[symmetric] RA2_true)
+  apply (simp add: RA1_def aseq_ades_def prefix_post_def
+      prefix_offer_post_def prefix_diverge_post_def
+      ades_state_choice_def expr_if_def rad_trace_extensions_def
+      fun_eq_iff Let_def lens_defs rad_state.wait_def astate.s_def
+      des_vars.more\<^sub>L_def true_pred_def disj_pred_def
+      conj_pred_def not_pred_def SEXP_def
+      subst_ext_def subst_app_def ex_in_conv[symmetric])
+  apply clarify
+  subgoal for x0 y0
+    apply (rule iffI)
+     apply (fastforce intro: order_trans)
+    apply (elim disjE bexE)
+     subgoal for y
+       apply (rule conjI)
+        apply (rule_tac x=y in bexI; fastforce)
+       by (rule_tac x=y in exI; fastforce)
+    subgoal for y
+      apply (rule conjI)
+       apply (rule_tac x="rad_state.wait\<^sub>v_update (\<lambda>_. False)
+           (rad_state.tr\<^sub>v_update
+             (\<lambda>_. rad_state.tr\<^sub>v (astate.s\<^sub>v (des_vars.more x0)) @ [a])
+             y)" in bexI; fastforce)
+      by (rule_tac x="rad_state.wait\<^sub>v_update (\<lambda>_. False)
+          (rad_state.tr\<^sub>v_update
+            (\<lambda>_. rad_state.tr\<^sub>v (astate.s\<^sub>v (des_vars.more x0)) @ [a])
+            y)" in exI; fastforce)
+    done
+  done
+
+(* Thesis Theorem T.5.4.29 instantiated to Chaos. *)
+lemma Prefix_Chaos_RAD_RA:
+  "(a \<rightarrow>\<^sub>R\<^sub>A\<^sub>D Chaos\<^sub>R\<^sub>A\<^sub>D) =
+   RA ((\<not> prefix_diverge_post a) \<turnstile>
+       (prefix_offer_post a \<or> prefix_diverge_post a))"
+proof -
+  have component_unrests:
+      "$ok\<^sup>> \<sharp> (true :: 'e reactive_angelic_design)"
+      "$ok\<^sup>> \<sharp> prefix_post a"
+      "$ok\<^sup>< \<sharp> (false :: 'e reactive_angelic_design)"
+      "$ok\<^sup>< \<sharp> (true :: 'e reactive_angelic_design)"
+    by (simp_all add: unrest)
+  have not_true_PBMH:
+      "(\<not> (true :: 'e reactive_angelic_design)) is PBMH_ades"
+    by (simp only: pred_ba.compl_top_eq false_PBMH_ades)
+  have prefix_PBMH: "prefix_post a is PBMH_ades"
+    by (simp add: Healthy_def')
+  have "(a \<rightarrow>\<^sub>R\<^sub>A\<^sub>D Chaos\<^sub>R\<^sub>A\<^sub>D) =
+      (RA (true \<turnstile> prefix_post a) ;;\<^sub>D\<^sub>A RA true)"
+    by (simp only: Prefix_RAD_def PrefixSkip_RAD_RA Chaos_RAD_RA)
+  also have "... =
+      RA ((\<not> prefix_diverge_post a) \<turnstile>
+          (prefix_offer_post a \<or> prefix_diverge_post a))"
+    using RA_design_seq[
+      where P=true and Q="prefix_post a" and R=false and S=true,
+      OF component_unrests not_true_PBMH prefix_PBMH]
+    by (simp only: design_false_pre pred_ba.compl_top_eq
+        pred_ba.compl_bot_eq pred_impl_laws RA1_false
+        aseq_ades_false_left prefix_handover_diverge
+        prefix_continuation_chaos pred_ba.inf_top_left)
+  finally show ?thesis .
+qed
+
+(* Paper Example 17 / Thesis Example 34: the angel avoids the
+   divergence following the event by choosing termination. *)
+lemma Prefix_Skip_Chaos_angelic_choice:
+  "(a \<rightarrow>\<^sub>R\<^sub>A\<^sub>D Skip\<^sub>R\<^sub>A\<^sub>D) \<squnion>\<^sub>R\<^sub>A\<^sub>D
+   (a \<rightarrow>\<^sub>R\<^sub>A\<^sub>D Chaos\<^sub>R\<^sub>A\<^sub>D) =
+   (a \<rightarrow>\<^sub>R\<^sub>A\<^sub>D Skip\<^sub>R\<^sub>A\<^sub>D)"
+proof -
+  have skip_absorb:
+      "(RA \<circ> A) (true \<turnstile> prefix_post a) =
+       RA (true \<turnstile> prefix_post a)"
+    by (rule RA_A_absorb_design_true; simp add: Healthy_def' unrest)
+  have chaos_PBMH:
+      "(\<not> (\<not> prefix_diverge_post a)) is PBMH_ades"
+    by (simp add: pred_ba.double_compl Healthy_def')
+  have chaos_absorb:
+      "(RA \<circ> A) ((\<not> prefix_diverge_post a) \<turnstile>
+          (prefix_offer_post a \<or> prefix_diverge_post a)) =
+       RA ((\<not> prefix_diverge_post a) \<turnstile>
+          (prefix_offer_post a \<or> prefix_diverge_post a))"
+    by (rule RA_A_absorb_design[OF chaos_PBMH])
+      (simp_all add: Healthy_def' PBMH_ades_disj unrest)
+  have "(a \<rightarrow>\<^sub>R\<^sub>A\<^sub>D Skip\<^sub>R\<^sub>A\<^sub>D) \<squnion>\<^sub>R\<^sub>A\<^sub>D
+      (a \<rightarrow>\<^sub>R\<^sub>A\<^sub>D Chaos\<^sub>R\<^sub>A\<^sub>D) =
+      (RA \<circ> A) (true \<turnstile> prefix_post a) \<squnion>
+      (RA \<circ> A) ((\<not> prefix_diverge_post a) \<turnstile>
+        (prefix_offer_post a \<or> prefix_diverge_post a))"
+    by (simp only: Prefix_Skip_RAD_RA Prefix_Chaos_RAD_RA
+        skip_absorb chaos_absorb)
+  also have "... = (RA \<circ> A)
+      ((true \<turnstile> prefix_post a) \<squnion>
+       ((\<not> prefix_diverge_post a) \<turnstile>
+        (prefix_offer_post a \<or> prefix_diverge_post a)))"
+    apply (rule RA_A_angelic_choice)
+       apply (simp add: Healthy_def' design_as_disj PBMH_ades_disj
+          PBMH_ades_conj_ok)
+      apply (simp add: Healthy_def' design_as_disj PBMH_ades_disj
+          PBMH_ades_conj_ok pred_ba.double_compl)
+     apply (rule design_is_H1_H2; simp add: unrest)
+    by (rule design_is_H1_H2; simp add: unrest)
+  also have "... = (RA \<circ> A) (true \<turnstile> prefix_post a)"
+    apply (rule arg_cong[where f="RA \<circ> A"])
+    apply (simp only: design_inf)
+    by (simp add: prefix_post_def expr_if_def rad_state.wait_def
+        SEXP_def lens_defs prefix_offer_post_def
+        prefix_diverge_post_def design_def fun_eq_iff Let_def;
+        pred_auto)
+  also have "... = (a \<rightarrow>\<^sub>R\<^sub>A\<^sub>D Skip\<^sub>R\<^sub>A\<^sub>D)"
+    by (simp only: Prefix_Skip_RAD_RA skip_absorb[symmetric])
+  finally show ?thesis .
+qed
+
+end
